theories/Sync.v
@@ -15,7 +15,7 @@ Definition dirty (g s: node) (p: path) : bool :=
 Definition replace (p: path) (s: node) : node -> node :=
   if cd p s is Some n then override p n else rmf p.
 
-(* Program *) Fixpoint recon (g a b: node) (* {measure (size g)} *) : node * node * node :=
+Program Fixpoint recon (g a b: node) {measure (size g)} : node * node * node :=
   if a =? g
   then (b, b, b)
   else
@@ -27,34 +27,50 @@ Definition replace (p: path) (s: node) : node -> node :=
       else
         match a, b with
         | Directory da, Directory db =>
-          let dg := if g is Directory dg then dg else [] in
-          let '(dg', da', db') :=
-              fold_left
-                (fun '(dg, da, db) f =>
+          let dg : mapping := if g is Directory dg then dg else [] in
+          let fgab :=
+              map
+                (fun f : string =>
                    match lookup f dg, lookup f da, lookup f db with
                    | Some g, Some a, Some b =>
-                     let '(g', a', b') := (g, a, b) in
-                     (* let '(g', a', b') := recon g a b in *)
-                     (add f g' dg, add f a' da, add f b' db)
+                     let '(g', a', b') := recon g a b in
+                     (add f g', add f a', add f b')
                    | None, Some a, Some b =>
                      if a =? b
-                     then (add f a dg, da, db)
-                     else (dg, da, db)
+                     then (add f a, id, id)
+                     else (id, id, id)
                    | Some g, Some a, None =>
                      if a =? g
-                     then (remove f dg, remove f da, db)
-                     else (dg, da, db)
+                     then (remove f, remove f, id)
+                     else (id, id, id)
                    | Some g, None, Some b =>
                      if b =? g
-                     then (remove f dg, da, remove f db)
-                     else (dg, da, db)
+                     then (remove f, id, remove f)
+                     else (id, id, id)
                    | None, None, Some b =>
-                     (add f b dg, add f b da, db)
+                     (add f b, add f b, id)
                    | None, Some a, None =>
-                     (add f a dg, da, add f a db)
+                     (add f a, id, add f a)
                    | _, None, None =>
-                     (remove f dg, da, db)
-                   end) (map fst $ da ++ db) (dg, da, db) in
+                     (remove f, id, id)
+                   end) (map fst $ da ++ db) in
+          let '(dg', da', db') :=
+              @fold_left (_ * _ * _) (_ * _ * _)
+                         (fun '(dg, da, db) '(fg, fa, fb) =>
+                           (fg dg, fa da, fb db)) fgab (dg, da, db) in
           (Directory dg', Directory da', Directory db')
         | _, _ => (g, a, b)
         end.
+Next Obligation.
+  destruct g0; try discriminate.
+  rewrite alist_find_alt in Heq_anonymous.
+  unfold alist_find' in Heq_anonymous.
+  unfold compose in Heq_anonymous.
+  destruct (find (fun x : string * node => RelDec.rel_dec f (fst x)) a0) eqn:Hfind;
+    try discriminate.
+  destruct p.
+  inversion Heq_anonymous; subst.
+  apply find_some in Hfind.
+  intuition.
+  eapply size_subdir; eauto.
+Defined.
